simulation/correct_get_start_addr.v
@@ -40,7 +40,7 @@ Section Get_start_addr.
 
   (* [match_arg] relates the Coq arguments and the C arguments *)
   Definition match_arg_list : DList.t (fun x => x -> val -> State.state -> Memory.Mem.mem -> Prop) args :=
-    (DList.DCons (match_region mrs_block)
+    (DList.DCons (match_region state_block mrs_block ins_block)
        (DList.DNil _)).
 
   (* [match_res] relates the Coq result and the C result *)
