simulation/correct_store_mem_reg.v
@@ -1,0 +1,171 @@
+From bpf.comm Require Import State Monad.
+From bpf.monadicmodel Require Import rBPFInterpreter.
+From Coq Require Import List Lia ZArith.
+From compcert Require Import Integers Values Clight Memory AST.
+Import ListNotations.
+
+From bpf.clight Require Import interpreter.
+
+From bpf.proof Require Import MatchState Clightlogic clight_exec CommonLemma CorrectRel.
+
+(**
+Check store_mem_reg.
+
+store_mem_reg
+     : memory_chunk -> val -> val -> M unit
+
+ *)
+
+Section Store_mem_reg.
+
+  (** The program contains our function of interest [fn] *)
+  Definition p : Clight.program := prog.
+
+  (* [Args,Res] provides the mapping between the Coq and the C types *)
+  (* Definition Args : list CompilableType := [stateCompilableType].*)
+  Definition args : list Type := [(memory_chunk:Type); val; val].
+  Definition res : Type := unit.
+
+  (* [f] is a Coq Monadic function with the right type *)
+  Definition f : arrow_type args (M res) := Monad.store_mem_reg.
+
+  Variable state_block: block. (**r a block storing all rbpf state information? *)
+  Variable mrs_block: block.
+  Variable ins_block: block.
+
+  Variable modifies : block. (* of the C code *)
+
+  (* [fn] is the Cligth function which has the same behaviour as [f] *)
+  Definition fn: Clight.function := f_store_mem_reg.
+
+  Definition stateM_correct (st:unit) (v: val) (stm:State.state) (m: Memory.Mem.mem) :=
+    v = Vptr state_block Ptrofs.zero /\ match_state state_block mrs_block ins_block stm m.
+
+  (* [match_arg] relates the Coq arguments and the C arguments *)
+  Definition match_arg_list : DList.t (fun x => x -> val -> State.state -> Memory.Mem.mem -> Prop) ((unit:Type) ::args) :=
+    DList.DCons stateM_correct
+      (DList.DCons (stateless match_chunk)
+         (DList.DCons (val_ptr_correct state_block mrs_block ins_block)
+            (DList.DCons (stateless val64_correct)
+              (DList.DNil _)))).
+
+  (* [match_res] relates the Coq result and the C result *)
+  Definition match_res : res -> val -> State.state -> Memory.Mem.mem -> Prop := fun x v st m => match_state state_block mrs_block ins_block st m /\ v = Vundef.
+
+  Instance correct_function3_store_mem_reg : forall a, correct_function3 p args res f fn [modifies] false match_arg_list match_res a.
+Proof.
+  correct_function_from_body args.
+  correct_body.
+  unfold f, store_mem_reg, State.store_mem_reg, Mem.storev, INV, app.
+  repeat intro.
+  get_invariant _st.
+  get_invariant _chunk.
+  get_invariant _addr.
+  get_invariant _v.
+  unfold stateM_correct in c2.
+  unfold stateless, match_chunk in c3.
+  unfold val_ptr_correct in c4.
+  unfold stateless, val64_correct in c5.
+  destruct c2 as (Hptr & Hmatch).
+  destruct c4 as (Hc0_eq & b & ofs & Hvalid_blk & Hc0_ptr & Hneq_blk).
+  destruct c5 as (Hc1_eq & vl & Hvl_eq).
+  subst.
+
+  unfold rBPFAST.memory_chunk_to_valu32, rBPFAST.well_chunk_Z in p1.
+  unfold match_res.
+(*
+  assert (Hstore_eq: Mem.store c (bpf_m st) b (Ptrofs.unsigned ofs) (vlong_to_vint_or_vlong c (Vlong vl)) = Mem.store c m b (Ptrofs.unsigned ofs) (vlong_to_vint_or_vlong c (Vlong vl))). {
+    eapply match_state_implies_store_equal; eauto.
+  }
+  rewrite Hstore_eq; clear Hstore_eq. *)
+  unfold vlong_to_vint_or_vlong.
+  destruct c; try constructor.
+  all: destruct Mem.store eqn: Hstore; [| constructor].
+  all: intros; exists Vundef; eexists; exists Events.E0.
+  - (**r c = Mint8unsigned *)
+    split.
+    forward_star.
+    change (Int.unsigned (Int.repr 1)) with 1%Z.
+    simpl.
+    unfold step2.
+    forward_star.
+    forward_star.
+    forward_star.
+    unfold Mem.storev.
+    simpl.
+    admit.
+    forward_star.
+    forward_star.
+    forward_star.
+    split.
+    split; [ |reflexivity].
+    admit.
+    split; [constructor | ].
+    admit.
+  - (**r c = Mint16unsigned *)
+    split.
+    forward_star.
+    change (Int.unsigned (Int.repr 2)) with 2%Z.
+    simpl.
+    unfold step2.
+    forward_star.
+    forward_star.
+    forward_star.
+    unfold Mem.storev.
+    simpl.
+    admit.
+    forward_star.
+    forward_star.
+    forward_star.
+    split.
+    split; [ |reflexivity].
+    admit.
+    split; [constructor | ].
+    admit.
+  - (**r c = Mint32 *)
+    split.
+    forward_star.
+    change (Int.unsigned (Int.repr 4)) with 4%Z.
+    simpl.
+    unfold step2.
+    forward_star.
+    forward_star.
+    forward_star.
+    unfold Mem.storev.
+    simpl.
+    admit.
+    forward_star.
+    forward_star.
+    forward_star.
+    split.
+    split; [ |reflexivity].
+    admit.
+    split; [constructor | ].
+    admit.
+  - (**r c = Mint64 *)
+    split.
+    forward_star.
+    change (Int.unsigned (Int.repr 8)) with 8%Z.
+    simpl.
+    unfold step2.
+    forward_star.
+    forward_star.
+    forward_star.
+    unfold Mem.storev.
+    simpl.
+    admit.
+    forward_star.
+    forward_star.
+    forward_star.
+    split.
+    split; [ |reflexivity].
+    admit.
+    split; [constructor | ].
+    admit.
+    Unshelve.
+    all: assumption.
+Qed.
+
+End Store_mem_reg.
+
+Existing Instance correct_function3_store_mem_reg.
